@prefix : <https://w3id.org/situannotate-dl#> .
@prefix dc: <http://purl.org/dc/elements/1.1/> .
@prefix owl: <http://www.w3.org/2002/07/owl#> .
@prefix rdf: <http://www.w3.org/1999/02/22-rdf-syntax-ns#> .
@prefix xml: <http://www.w3.org/XML/1998/namespace> .
@prefix xsd: <http://www.w3.org/2001/XMLSchema#> .
@prefix rdfs: <http://www.w3.org/2000/01/rdf-schema#> .
@prefix skos: <http://www.w3.org/2004/02/skos/core#> .
@prefix terms: <http://purl.org/dc/terms/> .
@prefix fschema: <https://w3id.org/framester/schema/> .
@prefix ontolex: <http://www.w3.org/ns/lemon/ontolex#> .
@prefix situannotate: <https://w3id.org/situannotate#> .

@base <https://w3id.org/situannotate-dl#> .

<https://w3id.org/situannotate-dl#> rdf:type owl:Ontology ;
                                 dc:creator "Delfina Sol Martinez Pandiani" ;
                                 rdfs:comment "This is the SituAnnotate ontology module for representing distributional linguistics (DL) annotation situations. It imports and specializes the core situAnnotate ontology." ;
                                 owl:imports <https://w3id.org/situannotate#> .


#################################################################
#    Object Properties
#################################################################

###  <https://w3id.org/situannotate-dl#hasCollocateTypedBy
:hasCollocateTypedBy rdf:type owl:ObjectProperty ;
                          rdfs:subPropertyOf situannotate:hasAnnotationTypedBy ;
                          owl:inverseOf :typesCollocateOf ;
                          rdfs:comment "Relates a concept with a concept that types one of its collocations." ;
                          rdfs:label "has collocate typed by" .


###  <https://w3id.org/situannotate-dl#typesCollocateOf
:typesCollocateOf rdf:type owl:ObjectProperty ;
                       rdfs:subPropertyOf situannotate:typesAnnotationOf ;
                       rdfs:domain situannotate:Concept ;
                       rdfs:range situannotate:Concept ;
                       rdfs:comment "Relates a concept with another concept that it collocates with." ;
                       rdfs:label "types collocate of" .



#################################################################
#    Classes
#################################################################

###  <https://w3id.org/situannotate-dl#CollocationAnnotation
:CollocationAnnotation rdf:type owl:Class ;
                            rdfs:subClassOf situannotate:Annotation ;
                            rdfs:comment "An annotation referring to a collocation." ;
                            rdfs:label "Collocation Annotation" .


###  <https://w3id.org/situannotate-dl#CollocationAnnotationDescription
:CollocationAnnotationDescription rdf:type owl:Class ;
                                       rdfs:subClassOf situannotate:AnnotationDescription ;
                                       rdfs:comment "A description of a collocation annotation, satisfied by a CollocationAnnotationSituation." ;
                                       rdfs:label "Collocation Annotation Description" .


###  <https://w3id.org/situannotate-dl#CollocationRole
:CollocationRole rdf:type owl:Class ;
                      rdfs:subClassOf situannotate:AnnotationRole ;
                      rdfs:comment "A role associated with collocation annotations." ;
                      rdfs:label "Collocation Role" .


###  <https://w3id.org/situannotate-dl#CollocationSituation
:CollocationSituation rdf:type owl:Class ;
                           rdfs:subClassOf situannotate:AnnotationSituation ;
                           rdfs:comment "A situation in which collocation annotation occurs." ;
                           rdfs:label "Collocation Situation" .
